theories/interop/wrapper_wp_ext_call_laws.v
@@ -315,6 +315,150 @@ Proof.
   iFrame. iPureIntro; split_and!; eauto. done.
 Qed.
 
+Lemma wp_ext_call_alloc : ext_call_is_sound WP_alloc_spec.
+Proof.
+  intros E T s vv K Ξ Φ.
+  rewrite weakestpre.wp_unfold. rewrite /weakestpre.wp_pre.
+  iIntros "%Hnone Hnb HT IH %σ Hσ".
+  SI_not_at_boundary. iNamed "HT". iNamed "HGC". SI_GC_agree.
+  pose (tg, repeat (Lint 0) (Z.to_nat sz)) as blk.
+  iAssert (⌜∀ k lv, roots_m !! k = Some lv →
+            ∃ w, mem !! k = Some (Storing w) ∧ repr_lval (θC ρc) lv w⌝)%I as "%Hroots".
+  1: { iIntros (kk vv Hroots).
+       iPoseProof (big_sepM_lookup with "GCrootspto") as "(%wr & Hwr & %Hw2)"; first done.
+       iExists wr. iSplit; last done. iApply (gen_heap_valid with "HσC Hwr"). }
+  destruct (make_repr (θC ρc) roots_m mem) as [privmem Hpriv]; try done.
+
+  iModIntro. iApply wp_pre_cases_c_prim; [done|by eauto|..].
+  { destruct (allocate_in_χ_priv_strong (dom (θC ρc)) (χC ρc) (Mut, blk) Hχinj) as (χC1&γ&HχC1&Hγθ).
+    pose (fresh (map_to_set (fun a b => b) (θC ρc) : gset loc)) as afresh.
+    pose (is_fresh (map_to_set (fun a b => b) (θC ρc) : gset loc)) as Hafresh.
+    do 3 eexists.
+    eapply (PrimAllocS _ tg sz roots_m ρc privmem mem γ afresh mem _ _ (<[γ := afresh]> (θC ρc))). 1,2,3,4: done. 2,3:reflexivity.
+    - destruct HχC1 as (_&(Hdisj&_)). eapply not_elem_of_dom.
+      erewrite dom_singleton_L in Hdisj. eapply disjoint_singleton_r. done.
+    - destruct HGCOK as [HGC1 HGC2]. split.
+      + intros k1 k2 v [[<- <-]|[H1L H1R]]%lookup_insert_Some [[??]|[H3L H3R]]%lookup_insert_Some.
+        1: done.
+        1: exfalso; eapply Hafresh; eapply elem_of_map_to_set;
+           do 2 eexists; split; first eapply H3R; done.
+        1: subst v; exfalso; eapply Hafresh; eapply elem_of_map_to_set;
+           do 2 eexists; split; first eapply H1R; done.
+        1: by eapply HGC1.
+      + rewrite dom_insert_L.
+        intros γ1 m1 tg1 vs1 γ' [->%elem_of_singleton|Hin]%elem_of_union [[Heq1 Heq2]%lookup_singleton_Some|[HluN Hlu]]%lookup_union_Some_raw Hγ';
+        eapply elem_of_union.
+        * injection Heq2; intros <- <- <-.
+          exfalso. eapply elem_of_list_In in Hγ'. eapply repeat_spec in Hγ'. congruence.
+        * rewrite lookup_singleton in HluN. done.
+        * subst γ1. injection Heq2; intros <- <- <-.
+          exfalso. eapply elem_of_list_In in Hγ'. eapply repeat_spec in Hγ'. congruence.
+        * right. destruct (Hfreezeρ) as [HHL HHR].
+          destruct ((ζσ ∪ ζvirt) !! γ1) as [[m2 [tg2 vs2]]|] eqn:Heq.
+          2: { exfalso. eapply not_elem_of_dom in Heq. eapply elem_of_dom_2 in Hlu.
+               rewrite HHL in Hlu; tauto. }
+          assert (vs2 = vs1) as ->.
+          1: { specialize (HHR _ _ _ Hlu Heq). inversion HHR; subst; done. }
+          eapply HGC2. 1: apply Hin. 2: apply Hγ'. apply Heq.
+    - eapply repr_mono. 2: done.
+      eapply insert_subseteq. by eapply not_elem_of_dom.
+    - intros a γ' HH1. rewrite dom_insert_L. eapply elem_of_union_r.
+      eapply Hrootslive. done.
+    - eapply lookup_insert. }
+
+
+
+  iIntros (w'' ρc' mem' Hstep) "!> !>". inversion Hstep.
+  simplify_eq. cbn.
+  assert (roots = roots_m ∧ privmem0 = privmem) as [-> ->].
+  { destruct H5 as (mm1 & H5). destruct Hpriv as (mm2 & Hpriv).
+    edestruct (repr_dom_eq (θC ρc) mem roots roots_m) as (Heq1&Heq2&Heq3).
+    1: rewrite H4 -H2; done.
+    1: apply HGCOK.
+    1-2: done. by subst. }
+
+  assert (χvirt !! γ = None) as Hγχ.
+  1: { eapply not_elem_of_dom.
+       destruct Hχvirt as [HHL HHR]. rewrite <- HHL.
+       by eapply not_elem_of_dom. }
+  assert (ζvirt !! γ = None) as Hγζv.
+  1: { eapply not_elem_of_dom. intros H.
+       eapply not_elem_of_dom in H6. apply H6.
+       destruct Hχvirt as [HHL HHR]. rewrite HHL.
+       eapply elem_of_weaken. 2: eapply Hother_blocks.
+       done. }
+  assert (ζσ !! γ = None) as Hγζσ.
+  1: { eapply not_elem_of_dom. intros H.
+       destruct Hstore_blocks as [HHL HHR]. apply HHR in H.
+       destruct H as (ℓ&Vs&Hχv&_). congruence. }
+  assert ((ζC ρc) !! γ = None) as HγζC.
+  1: { eapply not_elem_of_dom. destruct Hfreezeρ as [-> _].
+       rewrite dom_union_L. eapply not_elem_of_union;split;eapply not_elem_of_dom; done. }
+
+  assert (freeze_lstore ({[γ := (Mut, blk)]} ∪ ζC ρc) (ζσ ∪ <[γ:=(Mut, blk)]> ζvirt)) as Hfreezeρ_new.
+  { destruct Hfreezeρ as [HfL HfR]; split.
+    - rewrite !dom_union_L !dom_insert_L dom_empty_L. rewrite dom_union_L in HfL. clear -HfL. set_solver.
+    - rewrite <- insert_union_r. 2: done.
+      intros γ1 b1 b2 [[??]%lookup_singleton_Some|[??]]%lookup_union_Some_raw [[??]|[??]]%lookup_insert_Some; subst.
+      + econstructor.
+      + congruence.
+      + rewrite lookup_singleton in H. congruence.
+      + eapply HfR. all: done. }
+
+  iMod (set_to_none _ _ _ _ H5 with "HσC GCrootspto") as "(HσC&GCrootspto)".
+  iMod (set_to_some _ _ _ _ H10 with "HσC GCrootspto") as "(HσC&GCrootspto)".
+
+  iMod (ghost_var_update_halves with "GCζ SIζ") as "(GCζ&SIζ)".
+  iMod (ghost_var_update_halves with "GCχ SIχ") as "(GCχ&SIχ)".
+  iMod (ghost_var_update_halves with "GCθ SIθ") as "(GCθ&SIθ)".
+  
+  iMod (lstore_own_insert _ _ γ (Mut, blk) with "GCζvirt") as "(GCζvirt & Hbp1)"; first done.
+  iMod (lloc_own_allocate _ _ γ with "[] GCχvirt") as "(GCχvirt&Hbp2)"; first done.
+
+  iModIntro.
+  iSplitL "SIζ SIχ SIθ SIroots SIbound HnC HσC".
+  { iFrame; eauto. }
+  iApply ("IH" with "[-Hnb] Hnb").
+  iApply ("HWP" $! θC' γ with "[-Hbp2 Hbp1] [Hbp2 Hbp1] []"); try done.
+  3: iPureIntro; by econstructor.
+  2: iFrame; done.
+  rewrite /GC /named.
+  iExists _, _, (ζσ), (<[γ:=(Mut, blk)]> ζvirt), _, (<[γ:=LlocPrivate]> χvirt).
+  iExists σMLvirt, _, _, _. 
+  rewrite pub_locs_in_lstore_alloc_priv. 2: done. iFrame.
+  iPureIntro; split_and!; eauto.
+  2: destruct Hstore_blocks as [HsL HsR]; split.
+  - eapply map_disjoint_insert_r. split; done.
+  - intros ℓ Hdom. destruct (HsL ℓ Hdom) as (γ1 & Hγ1). exists γ1. rewrite lookup_insert_ne; first done.
+    intros ->; congruence.
+  - intros γ1; split.
+    + intros (ℓ&Vs&HH1&HH2)%HsR. exists ℓ,Vs; split; try done.
+      rewrite lookup_insert_ne; first done. intros ->; congruence.
+    + intros (ℓ&Vs&[[??]|[??]]%lookup_insert_Some&HH2); try congruence.
+      eapply HsR. by exists ℓ,Vs.
+  - erewrite !dom_insert_L. clear -Hother_blocks. set_solver.
+  - intros ℓ vs γ1 blk1 HH1 [[??]|[? HH2]]%lookup_insert_Some HH3; try congruence.
+    rewrite -!insert_union_r in HH3|-*; try done.
+    rewrite lookup_insert_ne in HH3; last done.
+    specialize (Hstore ℓ vs γ1 blk1 HH1 HH2 HH3).
+    inversion Hstore; subst. econstructor.
+    eapply Forall2_impl; first apply H0.
+    intros vml vl HH4. eapply is_val_mono. 3: apply HH4.
+    + eapply insert_subseteq. done.
+    + eapply insert_subseteq. eapply lookup_union_None; done.
+  - destruct Hχvirt as (HH1&HH2&HH3); unfold expose_llocs; split_and!.
+    + rewrite dom_insert_L. rewrite dom_union_L dom_singleton_L. by rewrite HH1.
+    + intros γ1 γ2 ℓ [[??]|[??]]%lookup_insert_Some [[??]|[??]]%lookup_insert_Some; subst; try congruence.
+      eapply HH2; done.
+    + intros γ0 v1 v2 [[??]%lookup_singleton_Some|[??]]%lookup_union_Some_raw [[??]|[??]]%lookup_insert_Some; subst; try congruence.
+      * econstructor.
+      * eapply HH3; done.
+  - intros γ1 γ2 ℓ [[??]%lookup_singleton_Some|[??]]%lookup_union_Some_raw [[??]%lookup_singleton_Some|[??]]%lookup_union_Some_raw;
+    subst; try congruence.
+    eapply Hχinj; done.
+  - eapply GC_correct_transport; done.
+Qed.
+
 Ltac solve_ext_call H := 
     iPoseProof (H with "[] Hnb H [IH]") as "Hwp"; [done
     | iIntros "!> %r HΞ Hnb"; iApply ("IH" with "HΞ Hnb"); by iApply "Hr"
@@ -327,14 +471,14 @@ Proof.
   intros E T s vv K Ξ Φ.
   rewrite weakestpre.wp_unfold. rewrite /weakestpre.wp_pre.
   iIntros "%Hnone Hnb HT IH %σ Hσ".
-  SI_not_at_boundary. cbn. iDestruct "HT" as "[H|[H|[H|[H|[H|H]]]]]".
+  SI_not_at_boundary. cbn. iDestruct "HT" as "[H|[H|[H|[H|[H|[H|H]]]]]]".
   - solve_ext_call wp_ext_call_int2val.
   - solve_ext_call wp_ext_call_val2int.
   - solve_ext_call wp_ext_call_registerroot.
   - solve_ext_call wp_ext_call_unregisterroot.
   - solve_ext_call wp_ext_call_modify.
   - solve_ext_call wp_ext_call_readfield.
-  (* - solve_ext_call wp_ext_call_alloc. *)
+  - solve_ext_call wp_ext_call_alloc.
 Qed.
 
 End Laws.
